Renaming and corrections in meta

lib/coq/OmnibigMeta.v
@@ -14,8 +14,11 @@ Section Omni_and_big_correction.
   Definition pc : Type := sVal -> Prop. (* postconditions *)
 
   Variable compile : sTrm -> tTrm.
-  Variable comp_values : sVal -> tVal.
-  Variable comp_values_inv : tVal -> sVal.
+
+  Variable Rval : sVal -> tVal -> Prop.
+
+  (* Variable comp_values : sVal -> tVal. *)
+  (* Variable comp_values_inv : tVal -> sVal. *)
 
   Definition bigstep (trm : Type) (val : Type) :=
     trm -> val -> Prop : Type.
@@ -30,34 +33,43 @@ Section Omni_and_big_correction.
     (t : trm) : Prop :=
     exists (v : val), exec t v.
 
+  Definition lift_R (R : sVal -> tVal -> Prop) : ((sVal -> Prop) -> tVal -> Prop) :=
+    fun P vt => exists vs, P vs /\ R vs vt.
 
   Hypothesis forward : forall (t : sTrm) (P : pc),
       sOmniBig t P ->
-      exists v, tBig (compile t) v /\ P (comp_values_inv v).
+      @terminates _ _ tBig (compile t) /\
+        (forall v, tBig (compile t) v -> lift_R Rval P v).
+
 
   Hypothesis omnibig_iff_terminates_and_correct : forall t P,
       sOmniBig t P <-> @terminates _ _ sBig t /\ forall v, sBig t v -> P v.
 
-  Hypothesis tBig_deter : forall t v v',
-      tBig t v -> tBig t v' -> v = v'.
+  (* Hypothesis tBig_deter : forall t v v', *)
+  (*     tBig t v -> tBig t v' -> v = v'. *)
 
   Lemma correction : forall (t : sTrm),
       @terminates _ _ sBig t ->
       @terminates _ _ tBig (compile t)
-      /\ forall v, tBig (compile t) v ->
-             exists P, sOmniBig t P /\ P (comp_values_inv v).
-  Proof using forward omnibig_iff_terminates_and_correct tBig_deter.
+      /\ forall vt, tBig (compile t) vt ->
+              exists vs, Rval vs vt /\ sBig t vs.
+      (* /\ forall v, tBig (compile t) v -> *)
+      (*        exists P, sOmniBig t P /\ P (comp_values_inv v). *)
+  Proof using forward omnibig_iff_terminates_and_correct.
     introv Hterm.
     specialize (@omnibig_iff_terminates_and_correct t (sp t)).
-    simpl in omnibig_iff_terminates_and_correct.
+    (* simpl in omnibig_iff_terminates_and_correct. *)
     assert (sOmniBig t (sp t)). now apply omnibig_iff_terminates_and_correct.
     specialize (@forward t (sp t) H).
-    destruct forward as (v'&HtBig&Hsp).
-    split; try solve [firstorder].
-    intros. exists (sp t). split; eauto.
-    forwards* : tBig_deter (compile t) v v'. congruence.
+    destruct forward as (Htermcomp&Hcomps).
+    unfold terminates in Htermcomp. destruct Htermcomp as (vt & Hvt).
+    split. unfold terminates. exists vt. apply Hvt.
+    intros. forwards * : Hcomps vt0 H0.
+    unfold lift_R in H1.
+    destruct H1 as (vs & Hvsinsp & HRv').
+    exists vs. split. auto.
+    apply Hvsinsp.
   Qed.
-
 
 
 
